ExistentialRules/ChaseSequence/Termination/MfaLike.lean
@@ -2,7 +2,8 @@ import BasicLeanDatastructures.List.Repeat
 
 import ExistentialRules.ChaseSequence.Termination.Basic
 import ExistentialRules.ChaseSequence.Termination.BacktrackingOfFacts
-import ExistentialRules.ChaseSequence.Termination.ConstantMappings
+import ExistentialRules.ChaseSequence.Termination.ConstantMappings.Basic
+import ExistentialRules.ChaseSequence.Termination.ConstantMappings.InterplayWithBacktracking
 import ExistentialRules.ChaseSequence.Termination.RenameConstantsApart
 import ExistentialRules.Terms.Cyclic
 
